
# Difference of Sums - Problem 2894

You are given positive integers `n` and `m`.

Define two integers as follows:

- `num1`: The sum of all integers in the range `[1, n]` that are **not divisible** by `m`.
- `num2`: The sum of all integers in the range `[1, n]` that **are divisible** by `m`.

Return the integer `num1 - num2`.

---

## Example 1

**Input:** `n = 10, m = 3`  
**Output:** `19`

**Explanation:**  
- Not divisible by 3: `[1,2,4,5,7,8,10]`, sum = 37  
- Divisible by 3: `[3,6,9]`, sum = 18  
- Difference: `37 - 18 = 19`

---

## Example 2

**Input:** `n = 5, m = 6`  
**Output:** `15`

**Explanation:**  
- Not divisible by 6: `[1,2,3,4,5]`, sum = 15  
- Divisible by 6: `[]`, sum = 0  
- Difference: `15 - 0 = 15`

---

## Example 3

**Input:** `n = 5, m = 1`  
**Output:** `-15`

**Explanation:**  
- Not divisible by 1: `[]`, sum = 0  
- Divisible by 1: `[1,2,3,4,5]`, sum = 15  
- Difference: `0 - 15 = -15`

---

## Formula

Let:
- `total_sum = n * (n + 1) / 2` (Sum of all integers from 1 to n)
- `k = n // m` (Number of terms divisible by m)
- `divisible_sum = m * k * (k + 1) / 2`

Then:
- `non_divisible_sum = total_sum - divisible_sum`
- **Result** = `non_divisible_sum - divisible_sum`

---

## Implementations

Various languages have been implemented:

- C++
- Java
- Python (2 & 3)
- C
- C#
- JavaScript / TypeScript / Node.js
- PHP
- Swift
- Kotlin
- Dart
- Go
- Ruby
- Scala
- Rust
- Racket
- Erlang
- Elixir

---

## Constraints

- `1 <= n, m <= 1000`

---

## Implementations

### C++

```cpp
class Solution {
public:
    int differenceOfSums(int n, int m) {
        int k = n / m;
        return n * (n + 1) / 2 - m * k * (k + 1) / 2 * 2;
    }
};
```

### Java

```java
class Solution {
    public int differenceOfSums(int n, int m) {
        int k = n / m;
        int totalSum = n * (n + 1) / 2;
        int divisibleSum = m * k * (k + 1) / 2;
        return totalSum - 2 * divisibleSum;
    }
}
```

### Python

```python
class Solution:
    def differenceOfSums(self, n: int, m: int) -> int:
        k = n // m
        total_sum = n * (n + 1) // 2
        divisible_sum = m * k * (k + 1) // 2
        non_divisible_sum = total_sum - divisible_sum
        return non_divisible_sum - divisible_sum
```

### Python 2

```python
class Solution(object):
    def differenceOfSums(self, n, m):
        k = n / m
        total_sum = n * (n + 1) / 2
        divisible_sum = m * k * (k + 1) / 2
        non_divisible_sum = total_sum - divisible_sum
        return non_divisible_sum - divisible_sum
```

### Python 3

```python
class Solution:
    def differenceOfSums(self, n: int, m: int) -> int:
        k = n // m
        total_sum = n * (n + 1) // 2
        divisible_sum = m * k * (k + 1) // 2
        non_divisible_sum = total_sum - divisible_sum
        return non_divisible_sum - divisible_sum
```

### C

```c
int differenceOfSums(int n, int m) {
    int k = n / m;
    int totalSum = n * (n + 1) / 2;
    int divisibleSum = m * k * (k + 1) / 2;
    return totalSum - 2 * divisibleSum;
}
```

### C#

```csharp
public class Solution {
    public int DifferenceOfSums(int n, int m) {
        int k = n / m;
        int totalSum = n * (n + 1) / 2;
        int divisibleSum = m * k * (k + 1) / 2;
        return totalSum - 2 * divisibleSum;
    }
}
```

### JavaScript

```javascript
var differenceOfSums = function(n, m) {
    let k = Math.floor(n / m);
    let totalSum = n * (n + 1) / 2;
    let divisibleSum = m * k * (k + 1) / 2;
    return totalSum - 2 * divisibleSum;
};
```

### TypeScript

```typescript
function differenceOfSums(n: number, m: number): number {
    const k = Math.floor(n / m);
    const totalSum = n * (n + 1) / 2;
    const divisibleSum = m * k * (k + 1) / 2;
    return totalSum - 2 * divisibleSum;
}
```

### PHP

```php
class Solution {
    function differenceOfSums($n, $m) {
        $k = intdiv($n, $m);
        $totalSum = intdiv($n * ($n + 1), 2);
        $divisibleSum = intdiv($m * $k * ($k + 1), 2);
        return $totalSum - 2 * $divisibleSum;
    }
}
```

### Swift

```swift
class Solution {
    func differenceOfSums(_ n: Int, _ m: Int) -> Int {
        let k = n / m
        let totalSum = n * (n + 1) / 2
        let divisibleSum = m * k * (k + 1) / 2
        return totalSum - 2 * divisibleSum
    }
}
```

### Kotlin

```kotlin
class Solution {
    fun differenceOfSums(n: Int, m: Int): Int {
        val k = n / m
        val totalSum = n * (n + 1) / 2
        val divisibleSum = m * k * (k + 1) / 2
        return totalSum - 2 * divisibleSum
    }
}
```

### Dart

```dart
class Solution {
  int differenceOfSums(int n, int m) {
    int k = n ~/ m;
    int totalSum = n * (n + 1) ~/ 2;
    int divisibleSum = m * k * (k + 1) ~/ 2;
    return totalSum - 2 * divisibleSum;
  }
}
```

### Go

```go
func differenceOfSums(n int, m int) int {
    k := n / m
    totalSum := n * (n + 1) / 2
    divisibleSum := m * k * (k + 1) / 2
    return totalSum - 2 * divisibleSum
}
```

### Ruby

```ruby
def difference_of_sums(n, m)
    k = n / m
    total_sum = n * (n + 1) / 2
    divisible_sum = m * k * (k + 1) / 2
    total_sum - 2 * divisible_sum
end
```

### Rust

```rust
impl Solution {
    pub fn difference_of_sums(n: i32, m: i32) -> i32 {
        let k = n / m;
        let total_sum = n * (n + 1) / 2;
        let divisible_sum = m * k * (k + 1) / 2;
        total_sum - 2 * divisible_sum
    }
}
```

### Scala

```scala
object Solution {
    def differenceOfSums(n: Int, m: Int): Int = {
        val k = n / m
        val totalSum = n * (n + 1) / 2
        val divisibleSum = m * k * (k + 1) / 2
        val nonDivisibleSum = totalSum - divisibleSum
        nonDivisibleSum - divisibleSum
    }
}
```

### Racket

```racket
(define/contract (difference-of-sums n m)
  (-> exact-integer? exact-integer? exact-integer?)
  (let* ([k (quotient n m)]
         [total-sum (/ (* n (+ n 1)) 2)]
         [divisible-sum (/ (* m k (+ k 1)) 2)])
    (- total-sum (* 2 divisible-sum))))
```

### Elixir

```elixir
defmodule Solution do
  @spec difference_of_sums(n :: integer, m :: integer) :: integer
  def difference_of_sums(n, m) do
    k = div(n, m)
    total_sum = div(n * (n + 1), 2)
    divisible_sum = div(m * k * (k + 1), 2)
    total_sum - 2 * divisible_sum
  end
end
```

### Erlang

```erlang
difference_of_sums(N, M) ->
    K = N div M,
    TotalSum = N * (N + 1) div 2,
    DivisibleSum = M * K * (K + 1) div 2,
    TotalSum - 2 * DivisibleSum.
```




